<?xml version="1.0"?>
<rdf:RDF xmlns="htp://purl.org/EnergyAlert/ontology#"
     xml:base="htp://purl.org/EnergyAlert/ontology"
     xmlns:schema="http://schema.org/"
     xmlns:ns="http://www.w3.org/2003/06/sw-vocab-status/ns#"
     xmlns:owl="http://www.w3.org/2002/07/owl#"
     xmlns:powder-s="http://www.w3.org/2007/05/powder-s#"
     xmlns:xsd="http://www.w3.org/2001/XMLSchema#"
     xmlns:voaf="http://purl.org/vocommons/voaf#"
     xmlns:skos="http://www.w3.org/2004/02/skos/core#"
     xmlns:rdfs="http://www.w3.org/2000/01/rdf-schema#"
     xmlns:ns1="http://creativecommons.org/ns#"
     xmlns:rdf="http://www.w3.org/1999/02/22-rdf-syntax-ns#"
     xmlns:terms="http://purl.org/dc/terms/"
     xmlns:xml="http://www.w3.org/XML/1998/namespace"
     xmlns:rec54="http://www.w3.org/2001/02pd/rec54#"
     xmlns:locn="http://www.w3.org/ns/locn#"
     xmlns:dcat="http://www.w3.org/ns/dcat#"
     xmlns:vann="http://purl.org/vocab/vann/"
     xmlns:foaf="http://xmlns.com/foaf/0.1/"
     xmlns:dc="http://purl.org/dc/elements/1.1/">
    <owl:Ontology rdf:about="htp://purl.org/EnergyAlert/ontology#"/>
    


    <!-- 
    ///////////////////////////////////////////////////////////////////////////////////////
    //
    // Annotation properties
    //
    ///////////////////////////////////////////////////////////////////////////////////////
     -->

    


    <!-- http://purl.org/dc/elements/1.1/contributor -->

    <owl:AnnotationProperty rdf:about="http://purl.org/dc/elements/1.1/contributor"/>
    


    <!-- http://purl.org/dc/elements/1.1/creator -->

    <owl:AnnotationProperty rdf:about="http://purl.org/dc/elements/1.1/creator"/>
    


    <!-- http://purl.org/dc/elements/1.1/date -->

    <owl:AnnotationProperty rdf:about="http://purl.org/dc/elements/1.1/date"/>
    


    <!-- http://purl.org/dc/elements/1.1/description -->

    <owl:AnnotationProperty rdf:about="http://purl.org/dc/elements/1.1/description"/>
    


    <!-- http://purl.org/dc/terms/identifier -->

    <owl:AnnotationProperty rdf:about="http://purl.org/dc/terms/identifier"/>
    


    <!-- http://www.w3.org/2003/06/sw-vocab-status/ns#term_status -->

    <owl:AnnotationProperty rdf:about="http://www.w3.org/2003/06/sw-vocab-status/ns#term_status"/>
    


    <!-- http://www.w3.org/2004/02/skos/core#definition -->

    <owl:AnnotationProperty rdf:about="http://www.w3.org/2004/02/skos/core#definition"/>
    


    <!-- http://www.w3.org/2004/02/skos/core#prefLabel -->

    <owl:AnnotationProperty rdf:about="http://www.w3.org/2004/02/skos/core#prefLabel"/>
    


    <!-- http://www.w3.org/2007/05/powder-s#describedby -->

    <owl:AnnotationProperty rdf:about="http://www.w3.org/2007/05/powder-s#describedby"/>
    


    <!-- 
    ///////////////////////////////////////////////////////////////////////////////////////
    //
    // Datatypes
    //
    ///////////////////////////////////////////////////////////////////////////////////////
     -->

    


    <!-- http://www.opengis.net/ont/geosparql#gmlLiteral -->

    <rdfs:Datatype rdf:about="http://www.opengis.net/ont/geosparql#gmlLiteral">
        <dc:contributor>Matthew Perry</dc:contributor>
        <dc:creator>OGC GeoSPARQL 1.0 Standard Working Group</dc:creator>
        <dc:date rdf:datatype="http://www.w3.org/2001/XMLSchema#date">2011-06-16</dc:date>
        <dc:description xml:lang="en">
      A GML serialization of a geometry object.
    </dc:description>
        <rdfs:comment xml:lang="en">
      A GML serialization of a geometry object.
    </rdfs:comment>
        <rdfs:isDefinedBy rdf:resource="http://www.opengis.net/ont/geosparql"/>
        <rdfs:isDefinedBy rdf:resource="http://www.opengis.net/spec/geosparql/1.0"/>
        <rdfs:label xml:lang="en">GML Literal</rdfs:label>
        <skos:definition xml:lang="en">
      A GML serialization of a geometry object.
    </skos:definition>
        <skos:prefLabel xml:lang="en">GML Literal</skos:prefLabel>
    </rdfs:Datatype>
    


    <!-- http://www.w3.org/2001/XMLSchema#date -->

    <rdfs:Datatype rdf:about="http://www.w3.org/2001/XMLSchema#date"/>
    


    <!-- 
    ///////////////////////////////////////////////////////////////////////////////////////
    //
    // Object Properties
    //
    ///////////////////////////////////////////////////////////////////////////////////////
     -->

    


    <!-- http://www.enexis.nl/IEC-CIM#Document.status -->

    <owl:ObjectProperty rdf:about="http://www.enexis.nl/IEC-CIM#Document.status">
        <rdfs:domain rdf:resource="http://www.enexis.nl/IEC-CIM#Document"/>
        <rdfs:range rdf:resource="http://www.enexis.nl/IEC-CIM#Status"/>
        <rdfs:comment>Status of subject matter (e.g., Agreement, Work) this document represents. For status of the document itself, use &apos;docStatus&apos; attribute.</rdfs:comment>
    </owl:ObjectProperty>
    


    <!-- http://www.enexis.nl/IEC-CIM#Incident_Location -->

    <owl:ObjectProperty rdf:about="http://www.enexis.nl/IEC-CIM#Incident_Location">
        <rdfs:domain rdf:resource="http://www.enexis.nl/IEC-CIM#Incident"/>
        <rdfs:range rdf:resource="http://www.enexis.nl/IEC-CIM#Location"/>
        <rdfs:comment>Incident at this location.Location of this incident.</rdfs:comment>
    </owl:ObjectProperty>
    


    <!-- http://www.enexis.nl/IEC-CIM#Location.mainAddress -->

    <owl:ObjectProperty rdf:about="http://www.enexis.nl/IEC-CIM#Location.mainAddress">
        <rdfs:domain rdf:resource="http://www.enexis.nl/IEC-CIM#Location"/>
        <rdfs:range rdf:resource="http://www.enexis.nl/IEC-CIM#StreetAddress"/>
        <rdfs:comment>Main address of the location.</rdfs:comment>
    </owl:ObjectProperty>
    


    <!-- http://www.enexis.nl/IEC-CIM#NameType_Names -->

    <owl:ObjectProperty rdf:about="http://www.enexis.nl/IEC-CIM#NameType_Names">
        <rdfs:domain rdf:resource="http://www.enexis.nl/IEC-CIM#Name"/>
        <rdfs:range rdf:resource="http://www.enexis.nl/IEC-CIM#NameType"/>
        <rdfs:comment>All names of this type.Type of this name.</rdfs:comment>
    </owl:ObjectProperty>
    


    <!-- http://www.enexis.nl/IEC-CIM#Names_IdentifiedObject -->

    <owl:ObjectProperty rdf:about="http://www.enexis.nl/IEC-CIM#Names_IdentifiedObject">
        <rdfs:domain rdf:resource="http://www.enexis.nl/IEC-CIM#Name"/>
        <rdfs:range rdf:resource="http://www.enexis.nl/IEC-CIM#IdentifiedObject"/>
        <rdfs:comment>All names of this identified object.Identified object that this name designates.</rdfs:comment>
    </owl:ObjectProperty>
    


    <!-- http://www.enexis.nl/IEC-CIM#Outage.actualPeriod -->

    <owl:ObjectProperty rdf:about="http://www.enexis.nl/IEC-CIM#Outage.actualPeriod">
        <rdfs:domain rdf:resource="http://www.enexis.nl/IEC-CIM#Outage"/>
        <rdfs:range rdf:resource="http://www.enexis.nl/IEC-CIM#DateTimeInterval"/>
        <rdfs:comment>Actual outage period; end of the period corresponds to the actual restoration time.</rdfs:comment>
    </owl:ObjectProperty>
    


    <!-- http://www.enexis.nl/IEC-CIM#Outage.estimatedPeriod -->

    <owl:ObjectProperty rdf:about="http://www.enexis.nl/IEC-CIM#Outage.estimatedPeriod">
        <rdfs:domain rdf:resource="http://www.enexis.nl/IEC-CIM#Outage"/>
        <rdfs:range rdf:resource="http://www.enexis.nl/IEC-CIM#DateTimeInterval"/>
        <rdfs:comment>Estimated outage period. The start of the period makes sense in case of a planned outage only, whereas the end of the period corresponds to the estimated restoration time in general.</rdfs:comment>
    </owl:ObjectProperty>
    


    <!-- http://www.enexis.nl/IEC-CIM#Outage.summary -->

    <owl:ObjectProperty rdf:about="http://www.enexis.nl/IEC-CIM#Outage.summary">
        <rdfs:domain rdf:resource="http://www.enexis.nl/IEC-CIM#Outage"/>
        <rdfs:range rdf:resource="http://www.enexis.nl/IEC-CIM#ServicePointOutageSummary"/>
        <rdfs:comment>Summary counts of service points (customers) affected by this outage.</rdfs:comment>
    </owl:ObjectProperty>
    


    <!-- http://www.enexis.nl/IEC-CIM#Outage_Incident -->

    <owl:ObjectProperty rdf:about="http://www.enexis.nl/IEC-CIM#Outage_Incident">
        <rdfs:domain rdf:resource="http://www.enexis.nl/IEC-CIM#Incident"/>
        <rdfs:range rdf:resource="http://www.enexis.nl/IEC-CIM#Outage"/>
        <rdfs:comment>Incident reported in trouble call that results in this outage.Outage for this incident.</rdfs:comment>
    </owl:ObjectProperty>
    


    <!-- http://www.enexis.nl/IEC-CIM#Outages_Equipments -->

    <owl:ObjectProperty rdf:about="http://www.enexis.nl/IEC-CIM#Outages_Equipments">
        <rdfs:domain rdf:resource="http://www.enexis.nl/IEC-CIM#Outage"/>
        <rdfs:range rdf:resource="http://www.enexis.nl/IEC-CIM#Equipment"/>
        <rdfs:comment>All outages in which this equipment is involved.All equipments associated with this outage.</rdfs:comment>
    </owl:ObjectProperty>
    


    <!-- http://www.enexis.nl/IEC-CIM#ServiceSupplier_UsagePoints -->

    <owl:ObjectProperty rdf:about="http://www.enexis.nl/IEC-CIM#ServiceSupplier_UsagePoints">
        <rdfs:domain rdf:resource="http://www.enexis.nl/IEC-CIM#ServiceSupplier"/>
        <rdfs:range rdf:resource="http://www.enexis.nl/IEC-CIM#UsagePoint"/>
        <rdfs:comment>ServiceSupplier (utility) utilising this usage point to deliver a service.All usage points this service supplier utilises to deliver a service.</rdfs:comment>
    </owl:ObjectProperty>
    


    <!-- http://www.enexis.nl/IEC-CIM#StreetAddress.streetDetail -->

    <owl:ObjectProperty rdf:about="http://www.enexis.nl/IEC-CIM#StreetAddress.streetDetail">
        <rdfs:domain rdf:resource="http://www.enexis.nl/IEC-CIM#StreetAddress"/>
        <rdfs:range rdf:resource="http://www.enexis.nl/IEC-CIM#StreetDetail"/>
        <rdfs:comment>Street detail.</rdfs:comment>
    </owl:ObjectProperty>
    


    <!-- http://www.enexis.nl/IEC-CIM#StreetAddress.townDetail -->

    <owl:ObjectProperty rdf:about="http://www.enexis.nl/IEC-CIM#StreetAddress.townDetail">
        <rdfs:domain rdf:resource="http://www.enexis.nl/IEC-CIM#StreetAddress"/>
        <rdfs:range rdf:resource="http://www.enexis.nl/IEC-CIM#TownDetail"/>
        <rdfs:comment>Town detail.</rdfs:comment>
    </owl:ObjectProperty>
    


    <!-- http://www.enexis.nl/IEC-CIM#UsagePoints_Outages -->

    <owl:ObjectProperty rdf:about="http://www.enexis.nl/IEC-CIM#UsagePoints_Outages">
        <rdfs:domain rdf:resource="http://www.enexis.nl/IEC-CIM#Outage"/>
        <rdfs:range rdf:resource="http://www.enexis.nl/IEC-CIM#UsagePoint"/>
        <rdfs:comment>All outages at this usage point.All usage points associated with this outage.</rdfs:comment>
    </owl:ObjectProperty>
    


    <!-- http://www.opengis.net/ont/geosparql#hasGeometry -->

    <owl:ObjectProperty rdf:about="http://www.opengis.net/ont/geosparql#hasGeometry">
        <rdfs:domain rdf:resource="http://www.opengis.net/ont/geosparql#Feature"/>
        <rdfs:range rdf:resource="http://www.opengis.net/ont/geosparql#Geometry"/>
        <dc:contributor>Matthew Perry</dc:contributor>
        <dc:creator>OGC GeoSPARQL 1.0 Standard Working Group</dc:creator>
        <dc:date rdf:datatype="http://www.w3.org/2001/XMLSchema#date">2011-06-16</dc:date>
        <dc:description xml:lang="en">
      A spatial representation for a given feature.
    </dc:description>
        <rdfs:comment xml:lang="en">
      A spatial representation for a given feature.
    </rdfs:comment>
        <rdfs:isDefinedBy rdf:resource="http://www.opengis.net/ont/geosparql"/>
        <rdfs:isDefinedBy rdf:resource="http://www.opengis.net/spec/geosparql/1.0"/>
        <rdfs:label xml:lang="en">hasGeometry</rdfs:label>
        <skos:definition xml:lang="en">
      A spatial representation for a given feature.
    </skos:definition>
        <skos:prefLabel xml:lang="en">hasGeometry</skos:prefLabel>
    </owl:ObjectProperty>
    


    <!-- 
    ///////////////////////////////////////////////////////////////////////////////////////
    //
    // Data properties
    //
    ///////////////////////////////////////////////////////////////////////////////////////
     -->

    


    <!-- http://www.enexis.nl/IEC-CIM#DateTimeInterval.end -->

    <owl:DatatypeProperty rdf:about="http://www.enexis.nl/IEC-CIM#DateTimeInterval.end">
        <rdfs:domain rdf:resource="http://www.enexis.nl/IEC-CIM#DateTimeInterval"/>
        <rdfs:range rdf:resource="http://www.w3.org/2001/XMLSchema#dateTimeStamp"/>
    </owl:DatatypeProperty>
    


    <!-- http://www.enexis.nl/IEC-CIM#DateTimeInterval.start -->

    <owl:DatatypeProperty rdf:about="http://www.enexis.nl/IEC-CIM#DateTimeInterval.start">
        <rdfs:domain rdf:resource="http://www.enexis.nl/IEC-CIM#DateTimeInterval"/>
        <rdfs:range rdf:resource="http://www.w3.org/2001/XMLSchema#dateTimeStamp"/>
    </owl:DatatypeProperty>
    


    <!-- http://www.enexis.nl/IEC-CIM#Document.createdDateTime -->

    <owl:DatatypeProperty rdf:about="http://www.enexis.nl/IEC-CIM#Document.createdDateTime">
        <rdfs:domain rdf:resource="http://www.enexis.nl/IEC-CIM#Document"/>
        <rdfs:range rdf:resource="http://www.w3.org/2001/XMLSchema#dateTime"/>
        <rdfs:comment>Date and time that this document was created.</rdfs:comment>
    </owl:DatatypeProperty>
    


    <!-- http://www.enexis.nl/IEC-CIM#Document.lastModifiedDateTime -->

    <owl:DatatypeProperty rdf:about="http://www.enexis.nl/IEC-CIM#Document.lastModifiedDateTime">
        <rdfs:domain rdf:resource="http://www.enexis.nl/IEC-CIM#Document"/>
        <rdfs:range rdf:resource="http://www.w3.org/2001/XMLSchema#dateTime"/>
        <rdfs:comment>Date and time this document was last modified. Documents may potentially be modified many times during their lifetime.</rdfs:comment>
    </owl:DatatypeProperty>
    


    <!-- http://www.enexis.nl/IEC-CIM#Document.title -->

    <owl:DatatypeProperty rdf:about="http://www.enexis.nl/IEC-CIM#Document.title">
        <rdfs:domain rdf:resource="http://www.enexis.nl/IEC-CIM#Document"/>
        <rdfs:range rdf:resource="http://www.w3.org/2001/XMLSchema#string"/>
    </owl:DatatypeProperty>
    


    <!-- http://www.enexis.nl/IEC-CIM#IdentifiedObject.description -->

    <owl:DatatypeProperty rdf:about="http://www.enexis.nl/IEC-CIM#IdentifiedObject.description">
        <rdfs:domain rdf:resource="http://www.enexis.nl/IEC-CIM#IdentifiedObject"/>
        <rdfs:range rdf:resource="http://www.w3.org/2001/XMLSchema#string"/>
        <rdfs:comment>The description is a free human readable text describing or naming the object. It may be non unique and may not correlate to a naming hierarchy.</rdfs:comment>
    </owl:DatatypeProperty>
    


    <!-- http://www.enexis.nl/IEC-CIM#IdentifiedObject.mRID -->

    <owl:DatatypeProperty rdf:about="http://www.enexis.nl/IEC-CIM#IdentifiedObject.mRID">
        <rdfs:domain rdf:resource="http://www.enexis.nl/IEC-CIM#IdentifiedObject"/>
        <rdfs:range rdf:resource="http://www.w3.org/2001/XMLSchema#string"/>
    </owl:DatatypeProperty>
    


    <!-- http://www.enexis.nl/IEC-CIM#IdentifiedObject.name -->

    <owl:DatatypeProperty rdf:about="http://www.enexis.nl/IEC-CIM#IdentifiedObject.name">
        <rdfs:domain rdf:resource="http://www.enexis.nl/IEC-CIM#IdentifiedObject"/>
        <rdfs:range rdf:resource="http://www.w3.org/2001/XMLSchema#string"/>
        <rdfs:comment>The name is any free human readable and possibly non unique text naming the object.</rdfs:comment>
    </owl:DatatypeProperty>
    


    <!-- http://www.enexis.nl/IEC-CIM#Name.name -->

    <owl:DatatypeProperty rdf:about="http://www.enexis.nl/IEC-CIM#Name.name">
        <rdfs:domain rdf:resource="http://www.enexis.nl/IEC-CIM#Name"/>
        <rdfs:range rdf:resource="http://www.w3.org/2001/XMLSchema#string"/>
        <rdfs:comment>Any free text that name the object.</rdfs:comment>
    </owl:DatatypeProperty>
    


    <!-- http://www.enexis.nl/IEC-CIM#NameType.name -->

    <owl:DatatypeProperty rdf:about="http://www.enexis.nl/IEC-CIM#NameType.name">
        <rdfs:domain rdf:resource="http://www.enexis.nl/IEC-CIM#NameType"/>
        <rdfs:range rdf:resource="http://www.w3.org/2001/XMLSchema#string"/>
        <rdfs:comment>Name of the name type.</rdfs:comment>
    </owl:DatatypeProperty>
    


    <!-- http://www.enexis.nl/IEC-CIM#Outage.cancelledDateTime -->

    <owl:DatatypeProperty rdf:about="http://www.enexis.nl/IEC-CIM#Outage.cancelledDateTime">
        <rdfs:domain rdf:resource="http://www.enexis.nl/IEC-CIM#Outage"/>
        <rdfs:range rdf:resource="http://www.w3.org/2001/XMLSchema#dateTime"/>
        <rdfs:comment>Date and time planned outage has been cancelled.</rdfs:comment>
    </owl:DatatypeProperty>
    


    <!-- http://www.enexis.nl/IEC-CIM#Outage.cause -->

    <owl:DatatypeProperty rdf:about="http://www.enexis.nl/IEC-CIM#Outage.cause">
        <rdfs:domain rdf:resource="http://www.enexis.nl/IEC-CIM#Outage"/>
        <rdfs:range rdf:resource="http://www.w3.org/2001/XMLSchema#string"/>
        <rdfs:comment>One or more causes of this outage.
Note: At present, this is a free text; could be replaced with a separate associated class in case we have multiple causes (e.g. OutageCauseType, inheriting from IdentifiedObject).</rdfs:comment>
    </owl:DatatypeProperty>
    


    <!-- http://www.enexis.nl/IEC-CIM#Outage.isPlanned -->

    <owl:DatatypeProperty rdf:about="http://www.enexis.nl/IEC-CIM#Outage.isPlanned">
        <rdfs:domain rdf:resource="http://www.enexis.nl/IEC-CIM#Outage"/>
        <rdfs:range rdf:resource="http://www.w3.org/2001/XMLSchema#boolean"/>
        <rdfs:comment>True if planned, false otherwise (for example due to a breaker trip).</rdfs:comment>
    </owl:DatatypeProperty>
    


    <!-- http://www.enexis.nl/IEC-CIM#ServicePointOutageSummary.totalCount -->

    <owl:DatatypeProperty rdf:about="http://www.enexis.nl/IEC-CIM#ServicePointOutageSummary.totalCount">
        <rdfs:domain rdf:resource="http://www.enexis.nl/IEC-CIM#ServicePointOutageSummary"/>
        <rdfs:range rdf:resource="http://www.w3.org/2001/XMLSchema#nonNegativeInteger"/>
        <rdfs:comment>Number of all service (delivery) points affected by an outage.</rdfs:comment>
    </owl:DatatypeProperty>
    


    <!-- http://www.enexis.nl/IEC-CIM#Status.value -->

    <owl:DatatypeProperty rdf:about="http://www.enexis.nl/IEC-CIM#Status.value">
        <rdfs:domain rdf:resource="http://www.enexis.nl/IEC-CIM#Status"/>
        <rdfs:range rdf:resource="http://www.w3.org/2001/XMLSchema#string"/>
        <rdfs:comment>Status value at &apos;dateTime&apos;; prior status changes may have been kept in instances of activity records associated with the object to which this status applies.</rdfs:comment>
    </owl:DatatypeProperty>
    


    <!-- http://www.enexis.nl/IEC-CIM#StreetAddress.postalCode -->

    <owl:DatatypeProperty rdf:about="http://www.enexis.nl/IEC-CIM#StreetAddress.postalCode">
        <rdfs:domain rdf:resource="http://www.enexis.nl/IEC-CIM#StreetAddress"/>
        <rdfs:range rdf:resource="http://www.w3.org/2001/XMLSchema#string"/>
        <rdfs:comment>Postal code for the address.</rdfs:comment>
    </owl:DatatypeProperty>
    


    <!-- http://www.enexis.nl/IEC-CIM#StreetDetail.name -->

    <owl:DatatypeProperty rdf:about="http://www.enexis.nl/IEC-CIM#StreetDetail.name">
        <rdfs:domain rdf:resource="http://www.enexis.nl/IEC-CIM#StreetDetail"/>
        <rdfs:range rdf:resource="http://www.w3.org/2001/XMLSchema#string"/>
        <rdfs:comment>Name of the street.</rdfs:comment>
    </owl:DatatypeProperty>
    


    <!-- http://www.enexis.nl/IEC-CIM#TownDetail.name -->

    <owl:DatatypeProperty rdf:about="http://www.enexis.nl/IEC-CIM#TownDetail.name">
        <rdfs:domain rdf:resource="http://www.enexis.nl/IEC-CIM#TownDetail"/>
        <rdfs:range rdf:resource="http://www.w3.org/2001/XMLSchema#string"/>
        <rdfs:comment>Town name.</rdfs:comment>
    </owl:DatatypeProperty>
    


    <!-- http://www.opengis.net/ont/geosparql#asGML -->

    <owl:DatatypeProperty rdf:about="http://www.opengis.net/ont/geosparql#asGML">
        <rdfs:subPropertyOf rdf:resource="http://www.opengis.net/ont/geosparql#hasSerialization"/>
        <rdfs:domain rdf:resource="http://www.opengis.net/ont/geosparql#Geometry"/>
        <rdfs:range rdf:resource="http://www.opengis.net/ont/geosparql#gmlLiteral"/>
        <dc:contributor>Matthew Perry</dc:contributor>
        <dc:creator>OGC GeoSPARQL 1.0 Standard Working Group</dc:creator>
        <dc:date rdf:datatype="http://www.w3.org/2001/XMLSchema#date">2011-06-16</dc:date>
        <dc:description xml:lang="en">
      The GML serialization of a geometry
    </dc:description>
        <rdfs:comment xml:lang="en">
      The GML serialization of a geometry
    </rdfs:comment>
        <rdfs:isDefinedBy rdf:resource="http://www.opengis.net/ont/geosparql"/>
        <rdfs:isDefinedBy rdf:resource="http://www.opengis.net/spec/geosparql/1.0"/>
        <rdfs:label xml:lang="en">asGML</rdfs:label>
        <skos:definition xml:lang="en">
      The GML serialization of a geometry
    </skos:definition>
        <skos:prefLabel xml:lang="en">asGML</skos:prefLabel>
    </owl:DatatypeProperty>
    


    <!-- http://www.opengis.net/ont/geosparql#hasSerialization -->

    <owl:DatatypeProperty rdf:about="http://www.opengis.net/ont/geosparql#hasSerialization">
        <rdfs:domain rdf:resource="http://www.opengis.net/ont/geosparql#Geometry"/>
        <rdfs:range rdf:resource="http://www.w3.org/2000/01/rdf-schema#Literal"/>
        <dc:contributor>Matthew Perry</dc:contributor>
        <dc:creator>OGC GeoSPARQL 1.0 Standard Working Group</dc:creator>
        <dc:date rdf:datatype="http://www.w3.org/2001/XMLSchema#date">2011-06-16</dc:date>
        <dc:description xml:lang="en">
      Connects a geometry object with its text-based serialization.
    </dc:description>
        <rdfs:comment xml:lang="en">
      Connects a geometry object with its text-based serialization.
    </rdfs:comment>
        <rdfs:isDefinedBy rdf:resource="http://www.opengis.net/ont/geosparql"/>
        <rdfs:isDefinedBy rdf:resource="http://www.opengis.net/spec/geosparql/1.0"/>
        <rdfs:label xml:lang="en">has serialization</rdfs:label>
        <skos:definition xml:lang="en">
      Connects a geometry object with its text-based serialization.
    </skos:definition>
        <skos:prefLabel xml:lang="en">has serialization</skos:prefLabel>
    </owl:DatatypeProperty>
    


    <!-- http://www.w3.org/ns/locn#thoroughfare -->

    <owl:DatatypeProperty rdf:about="http://www.w3.org/ns/locn#thoroughfare">
        <rdfs:range rdf:resource="http://www.w3.org/2000/01/rdf-schema#Literal"/>
        <terms:identifier rdf:datatype="http://www.w3.org/2001/XMLSchema#string">locn:thoroughfare</terms:identifier>
        <rdfs:comment xml:lang="en">An address component that represents the name of a passage or way through from one location to another. A thoroughfare is not necessarily a road, it might be a waterway or some other feature. The domain of locn:thoroughfare is locn:Address.</rdfs:comment>
        <rdfs:isDefinedBy rdf:resource="http://www.w3.org/ns/locn"/>
        <rdfs:label xml:lang="en">thoroughfare</rdfs:label>
        <ns:term_status xml:lang="en">testing</ns:term_status>
    </owl:DatatypeProperty>
    


    <!-- 
    ///////////////////////////////////////////////////////////////////////////////////////
    //
    // Classes
    //
    ///////////////////////////////////////////////////////////////////////////////////////
     -->

    


    <!-- http://www.enexis.nl/IEC-CIM#DateTimeInterval -->

    <owl:Class rdf:about="http://www.enexis.nl/IEC-CIM#DateTimeInterval">
        <owl:equivalentClass>
            <owl:Restriction>
                <owl:onProperty rdf:resource="http://www.enexis.nl/IEC-CIM#DateTimeInterval.end"/>
                <owl:minQualifiedCardinality rdf:datatype="http://www.w3.org/2001/XMLSchema#nonNegativeInteger">0</owl:minQualifiedCardinality>
                <owl:onDataRange rdf:resource="http://www.w3.org/2001/XMLSchema#dateTime"/>
            </owl:Restriction>
        </owl:equivalentClass>
        <owl:equivalentClass>
            <owl:Restriction>
                <owl:onProperty rdf:resource="http://www.enexis.nl/IEC-CIM#DateTimeInterval.start"/>
                <owl:minQualifiedCardinality rdf:datatype="http://www.w3.org/2001/XMLSchema#nonNegativeInteger">0</owl:minQualifiedCardinality>
                <owl:onDataRange rdf:resource="http://www.w3.org/2001/XMLSchema#dateTime"/>
            </owl:Restriction>
        </owl:equivalentClass>
        <owl:equivalentClass>
            <owl:Restriction>
                <owl:onProperty rdf:resource="http://www.enexis.nl/IEC-CIM#DateTimeInterval.end"/>
                <owl:maxQualifiedCardinality rdf:datatype="http://www.w3.org/2001/XMLSchema#nonNegativeInteger">1</owl:maxQualifiedCardinality>
                <owl:onDataRange rdf:resource="http://www.w3.org/2001/XMLSchema#dateTime"/>
            </owl:Restriction>
        </owl:equivalentClass>
        <owl:equivalentClass>
            <owl:Restriction>
                <owl:onProperty rdf:resource="http://www.enexis.nl/IEC-CIM#DateTimeInterval.start"/>
                <owl:maxQualifiedCardinality rdf:datatype="http://www.w3.org/2001/XMLSchema#nonNegativeInteger">1</owl:maxQualifiedCardinality>
                <owl:onDataRange rdf:resource="http://www.w3.org/2001/XMLSchema#dateTime"/>
            </owl:Restriction>
        </owl:equivalentClass>
        <rdfs:comment>Interval between two date and time points.</rdfs:comment>
    </owl:Class>
    


    <!-- http://www.enexis.nl/IEC-CIM#Document -->

    <owl:Class rdf:about="http://www.enexis.nl/IEC-CIM#Document">
        <rdfs:subClassOf rdf:resource="http://www.enexis.nl/IEC-CIM#IdentifiedObject"/>
        <rdfs:comment>Parent class for different groupings of information collected and managed as a part of a business process. It will frequently contain references to other objects, such as assets, people and power system resources.</rdfs:comment>
    </owl:Class>
    


    <!-- http://www.enexis.nl/IEC-CIM#Equipment -->

    <owl:Class rdf:about="http://www.enexis.nl/IEC-CIM#Equipment">
        <rdfs:subClassOf rdf:resource="http://www.enexis.nl/IEC-CIM#PowerSystemResource"/>
        <rdfs:comment>The parts of a power system that are physical devices, electronic or mechanical.</rdfs:comment>
    </owl:Class>
    


    <!-- http://www.enexis.nl/IEC-CIM#IdentifiedObject -->

    <owl:Class rdf:about="http://www.enexis.nl/IEC-CIM#IdentifiedObject">
        <rdfs:comment>This is a root class to provide common identification for all classes needing identification and naming attributes.</rdfs:comment>
    </owl:Class>
    


    <!-- http://www.enexis.nl/IEC-CIM#Incident -->

    <owl:Class rdf:about="http://www.enexis.nl/IEC-CIM#Incident">
        <rdfs:subClassOf rdf:resource="http://www.enexis.nl/IEC-CIM#Document"/>
        <rdfs:comment>Description of a problem in the field that may be reported in a trouble ticket or come from another source. It may have to do with an outage.</rdfs:comment>
    </owl:Class>
    


    <!-- http://www.enexis.nl/IEC-CIM#Location -->

    <owl:Class rdf:about="http://www.enexis.nl/IEC-CIM#Location">
        <owl:equivalentClass>
            <owl:Restriction>
                <owl:onProperty rdf:resource="http://www.enexis.nl/IEC-CIM#Location.mainAddress"/>
                <owl:minQualifiedCardinality rdf:datatype="http://www.w3.org/2001/XMLSchema#nonNegativeInteger">0</owl:minQualifiedCardinality>
                <owl:onClass rdf:resource="http://www.enexis.nl/IEC-CIM#StreetAddress"/>
            </owl:Restriction>
        </owl:equivalentClass>
        <owl:equivalentClass>
            <owl:Restriction>
                <owl:onProperty rdf:resource="http://www.enexis.nl/IEC-CIM#Location.mainAddress"/>
                <owl:maxQualifiedCardinality rdf:datatype="http://www.w3.org/2001/XMLSchema#nonNegativeInteger">1</owl:maxQualifiedCardinality>
                <owl:onClass rdf:resource="http://www.enexis.nl/IEC-CIM#StreetAddress"/>
            </owl:Restriction>
        </owl:equivalentClass>
        <rdfs:subClassOf rdf:resource="http://www.enexis.nl/IEC-CIM#IdentifiedObject"/>
        <rdfs:subClassOf rdf:resource="http://www.opengis.net/ont/geosparql#Feature"/>
        <rdfs:comment>The place, scene, or point of something where someone or something has been, is, and/or will be at a given moment in time. It can be defined with one or more postition points (coordinates) in a given coordinate system.</rdfs:comment>
    </owl:Class>
    


    <!-- http://www.enexis.nl/IEC-CIM#Name -->

    <owl:Class rdf:about="http://www.enexis.nl/IEC-CIM#Name"/>
    


    <!-- http://www.enexis.nl/IEC-CIM#NameType -->

    <owl:Class rdf:about="http://www.enexis.nl/IEC-CIM#NameType"/>
    


    <!-- http://www.enexis.nl/IEC-CIM#OrganisationRole -->

    <owl:Class rdf:about="http://www.enexis.nl/IEC-CIM#OrganisationRole">
        <rdfs:subClassOf rdf:resource="http://www.enexis.nl/IEC-CIM#IdentifiedObject"/>
        <rdfs:comment>Identifies a way in which an organisation may participate in the utility enterprise (e.g., customer, manufacturer, etc).</rdfs:comment>
    </owl:Class>
    


    <!-- http://www.enexis.nl/IEC-CIM#Outage -->

    <owl:Class rdf:about="http://www.enexis.nl/IEC-CIM#Outage">
        <owl:equivalentClass>
            <owl:Restriction>
                <owl:onProperty rdf:resource="http://www.enexis.nl/IEC-CIM#Outage.actualPeriod"/>
                <owl:minQualifiedCardinality rdf:datatype="http://www.w3.org/2001/XMLSchema#nonNegativeInteger">0</owl:minQualifiedCardinality>
                <owl:onClass rdf:resource="http://www.enexis.nl/IEC-CIM#DateTimeInterval"/>
            </owl:Restriction>
        </owl:equivalentClass>
        <owl:equivalentClass>
            <owl:Restriction>
                <owl:onProperty rdf:resource="http://www.enexis.nl/IEC-CIM#Outage.estimatedPeriod"/>
                <owl:minQualifiedCardinality rdf:datatype="http://www.w3.org/2001/XMLSchema#nonNegativeInteger">0</owl:minQualifiedCardinality>
                <owl:onClass rdf:resource="http://www.enexis.nl/IEC-CIM#DateTimeInterval"/>
            </owl:Restriction>
        </owl:equivalentClass>
        <owl:equivalentClass>
            <owl:Restriction>
                <owl:onProperty rdf:resource="http://www.enexis.nl/IEC-CIM#Outage.summary"/>
                <owl:minQualifiedCardinality rdf:datatype="http://www.w3.org/2001/XMLSchema#nonNegativeInteger">0</owl:minQualifiedCardinality>
                <owl:onClass rdf:resource="http://www.enexis.nl/IEC-CIM#ServicePointOutageSummary"/>
            </owl:Restriction>
        </owl:equivalentClass>
        <owl:equivalentClass>
            <owl:Restriction>
                <owl:onProperty rdf:resource="http://www.enexis.nl/IEC-CIM#Outage.actualPeriod"/>
                <owl:maxQualifiedCardinality rdf:datatype="http://www.w3.org/2001/XMLSchema#nonNegativeInteger">1</owl:maxQualifiedCardinality>
                <owl:onClass rdf:resource="http://www.enexis.nl/IEC-CIM#DateTimeInterval"/>
            </owl:Restriction>
        </owl:equivalentClass>
        <owl:equivalentClass>
            <owl:Restriction>
                <owl:onProperty rdf:resource="http://www.enexis.nl/IEC-CIM#Outage.estimatedPeriod"/>
                <owl:maxQualifiedCardinality rdf:datatype="http://www.w3.org/2001/XMLSchema#nonNegativeInteger">1</owl:maxQualifiedCardinality>
                <owl:onClass rdf:resource="http://www.enexis.nl/IEC-CIM#DateTimeInterval"/>
            </owl:Restriction>
        </owl:equivalentClass>
        <owl:equivalentClass>
            <owl:Restriction>
                <owl:onProperty rdf:resource="http://www.enexis.nl/IEC-CIM#Outage.summary"/>
                <owl:maxQualifiedCardinality rdf:datatype="http://www.w3.org/2001/XMLSchema#nonNegativeInteger">1</owl:maxQualifiedCardinality>
                <owl:onClass rdf:resource="http://www.enexis.nl/IEC-CIM#ServicePointOutageSummary"/>
            </owl:Restriction>
        </owl:equivalentClass>
        <owl:equivalentClass>
            <owl:Restriction>
                <owl:onProperty rdf:resource="http://www.enexis.nl/IEC-CIM#Outage.cancelledDateTime"/>
                <owl:minQualifiedCardinality rdf:datatype="http://www.w3.org/2001/XMLSchema#nonNegativeInteger">0</owl:minQualifiedCardinality>
                <owl:onDataRange rdf:resource="http://www.w3.org/2001/XMLSchema#dateTime"/>
            </owl:Restriction>
        </owl:equivalentClass>
        <owl:equivalentClass>
            <owl:Restriction>
                <owl:onProperty rdf:resource="http://www.enexis.nl/IEC-CIM#Outage.cause"/>
                <owl:minQualifiedCardinality rdf:datatype="http://www.w3.org/2001/XMLSchema#nonNegativeInteger">0</owl:minQualifiedCardinality>
                <owl:onDataRange rdf:resource="http://www.w3.org/2001/XMLSchema#string"/>
            </owl:Restriction>
        </owl:equivalentClass>
        <owl:equivalentClass>
            <owl:Restriction>
                <owl:onProperty rdf:resource="http://www.enexis.nl/IEC-CIM#Outage.isPlanned"/>
                <owl:minQualifiedCardinality rdf:datatype="http://www.w3.org/2001/XMLSchema#nonNegativeInteger">0</owl:minQualifiedCardinality>
                <owl:onDataRange rdf:resource="http://www.w3.org/2001/XMLSchema#boolean"/>
            </owl:Restriction>
        </owl:equivalentClass>
        <owl:equivalentClass>
            <owl:Restriction>
                <owl:onProperty rdf:resource="http://www.enexis.nl/IEC-CIM#Outage.cancelledDateTime"/>
                <owl:maxQualifiedCardinality rdf:datatype="http://www.w3.org/2001/XMLSchema#nonNegativeInteger">1</owl:maxQualifiedCardinality>
                <owl:onDataRange rdf:resource="http://www.w3.org/2001/XMLSchema#dateTime"/>
            </owl:Restriction>
        </owl:equivalentClass>
        <owl:equivalentClass>
            <owl:Restriction>
                <owl:onProperty rdf:resource="http://www.enexis.nl/IEC-CIM#Outage.cause"/>
                <owl:maxQualifiedCardinality rdf:datatype="http://www.w3.org/2001/XMLSchema#nonNegativeInteger">1</owl:maxQualifiedCardinality>
                <owl:onDataRange rdf:resource="http://www.w3.org/2001/XMLSchema#string"/>
            </owl:Restriction>
        </owl:equivalentClass>
        <owl:equivalentClass>
            <owl:Restriction>
                <owl:onProperty rdf:resource="http://www.enexis.nl/IEC-CIM#Outage.isPlanned"/>
                <owl:maxQualifiedCardinality rdf:datatype="http://www.w3.org/2001/XMLSchema#nonNegativeInteger">1</owl:maxQualifiedCardinality>
                <owl:onDataRange rdf:resource="http://www.w3.org/2001/XMLSchema#boolean"/>
            </owl:Restriction>
        </owl:equivalentClass>
        <rdfs:subClassOf rdf:resource="http://www.enexis.nl/IEC-CIM#Document"/>
        <rdfs:comment>Document describing details of an active or planned outage in a part of the electrical network.
A non-planned outage may be created upon:
- a breaker trip,
- a fault indicator status change,
- a meter event indicating customer outage,
- a reception of one or more customer trouble calls, or
- an operator command, reflecting information obtained from the field crew.
Outage restoration may be performed using a switching plan which complements the outage information with detailed switching activities, including the relationship to the crew and work.
A planned outage may be created upon:
- a request for service, maintenance or construction work in the field, or
- an operator-defined outage for what-if/contingency network analysis.</rdfs:comment>
    </owl:Class>
    


    <!-- http://www.enexis.nl/IEC-CIM#PowerSystemResource -->

    <owl:Class rdf:about="http://www.enexis.nl/IEC-CIM#PowerSystemResource">
        <rdfs:subClassOf rdf:resource="http://www.enexis.nl/IEC-CIM#IdentifiedObject"/>
        <rdfs:subClassOf rdf:resource="http://www.opengis.net/ont/geosparql#Feature"/>
        <rdfs:comment>A power system resource can be an item of equipment such as a switch, an equipment container containing many individual items of equipment such as a substation, or an organisational entity such as sub-control area. Power system resources can have measurements associated.</rdfs:comment>
    </owl:Class>
    


    <!-- http://www.enexis.nl/IEC-CIM#ServicePointOutageSummary -->

    <owl:Class rdf:about="http://www.enexis.nl/IEC-CIM#ServicePointOutageSummary">
        <owl:equivalentClass>
            <owl:Restriction>
                <owl:onProperty rdf:resource="http://www.enexis.nl/IEC-CIM#ServicePointOutageSummary.totalCount"/>
                <owl:minQualifiedCardinality rdf:datatype="http://www.w3.org/2001/XMLSchema#nonNegativeInteger">0</owl:minQualifiedCardinality>
                <owl:onDataRange rdf:resource="http://www.w3.org/2001/XMLSchema#nonNegativeInteger"/>
            </owl:Restriction>
        </owl:equivalentClass>
        <owl:equivalentClass>
            <owl:Restriction>
                <owl:onProperty rdf:resource="http://www.enexis.nl/IEC-CIM#ServicePointOutageSummary.totalCount"/>
                <owl:maxQualifiedCardinality rdf:datatype="http://www.w3.org/2001/XMLSchema#nonNegativeInteger">1</owl:maxQualifiedCardinality>
                <owl:onDataRange rdf:resource="http://www.w3.org/2001/XMLSchema#nonNegativeInteger"/>
            </owl:Restriction>
        </owl:equivalentClass>
        <rdfs:subClassOf rdf:resource="http://www.opengis.net/ont/geosparql#Feature"/>
        <rdfs:comment>Summary counts of service points affected by an outage. These counts are sometimes referred to as total and critical customer count.</rdfs:comment>
    </owl:Class>
    


    <!-- http://www.enexis.nl/IEC-CIM#ServiceSupplier -->

    <owl:Class rdf:about="http://www.enexis.nl/IEC-CIM#ServiceSupplier">
        <rdfs:subClassOf rdf:resource="http://www.enexis.nl/IEC-CIM#OrganisationRole"/>
        <rdfs:comment>Organisation that provides services to customers.</rdfs:comment>
    </owl:Class>
    


    <!-- http://www.enexis.nl/IEC-CIM#Status -->

    <owl:Class rdf:about="http://www.enexis.nl/IEC-CIM#Status">
        <owl:equivalentClass>
            <owl:Restriction>
                <owl:onProperty rdf:resource="http://www.enexis.nl/IEC-CIM#Status.value"/>
                <owl:minQualifiedCardinality rdf:datatype="http://www.w3.org/2001/XMLSchema#nonNegativeInteger">0</owl:minQualifiedCardinality>
                <owl:onDataRange rdf:resource="http://www.w3.org/2001/XMLSchema#string"/>
            </owl:Restriction>
        </owl:equivalentClass>
        <owl:equivalentClass>
            <owl:Restriction>
                <owl:onProperty rdf:resource="http://www.enexis.nl/IEC-CIM#Status.value"/>
                <owl:maxQualifiedCardinality rdf:datatype="http://www.w3.org/2001/XMLSchema#nonNegativeInteger">1</owl:maxQualifiedCardinality>
                <owl:onDataRange rdf:resource="http://www.w3.org/2001/XMLSchema#string"/>
            </owl:Restriction>
        </owl:equivalentClass>
        <rdfs:comment>Current status information relevant to an entity.</rdfs:comment>
    </owl:Class>
    


    <!-- http://www.enexis.nl/IEC-CIM#StreetAddress -->

    <owl:Class rdf:about="http://www.enexis.nl/IEC-CIM#StreetAddress">
        <owl:equivalentClass>
            <owl:Restriction>
                <owl:onProperty rdf:resource="http://www.enexis.nl/IEC-CIM#StreetAddress.streetDetail"/>
                <owl:minQualifiedCardinality rdf:datatype="http://www.w3.org/2001/XMLSchema#nonNegativeInteger">0</owl:minQualifiedCardinality>
                <owl:onClass rdf:resource="http://www.enexis.nl/IEC-CIM#StreetDetail"/>
            </owl:Restriction>
        </owl:equivalentClass>
        <owl:equivalentClass>
            <owl:Restriction>
                <owl:onProperty rdf:resource="http://www.enexis.nl/IEC-CIM#StreetAddress.townDetail"/>
                <owl:minQualifiedCardinality rdf:datatype="http://www.w3.org/2001/XMLSchema#nonNegativeInteger">0</owl:minQualifiedCardinality>
                <owl:onClass rdf:resource="http://www.enexis.nl/IEC-CIM#TownDetail"/>
            </owl:Restriction>
        </owl:equivalentClass>
        <owl:equivalentClass>
            <owl:Restriction>
                <owl:onProperty rdf:resource="http://www.enexis.nl/IEC-CIM#StreetAddress.streetDetail"/>
                <owl:maxQualifiedCardinality rdf:datatype="http://www.w3.org/2001/XMLSchema#nonNegativeInteger">1</owl:maxQualifiedCardinality>
                <owl:onClass rdf:resource="http://www.enexis.nl/IEC-CIM#StreetDetail"/>
            </owl:Restriction>
        </owl:equivalentClass>
        <owl:equivalentClass>
            <owl:Restriction>
                <owl:onProperty rdf:resource="http://www.enexis.nl/IEC-CIM#StreetAddress.townDetail"/>
                <owl:maxQualifiedCardinality rdf:datatype="http://www.w3.org/2001/XMLSchema#nonNegativeInteger">1</owl:maxQualifiedCardinality>
                <owl:onClass rdf:resource="http://www.enexis.nl/IEC-CIM#TownDetail"/>
            </owl:Restriction>
        </owl:equivalentClass>
        <owl:equivalentClass>
            <owl:Restriction>
                <owl:onProperty rdf:resource="http://www.enexis.nl/IEC-CIM#StreetAddress.postalCode"/>
                <owl:minQualifiedCardinality rdf:datatype="http://www.w3.org/2001/XMLSchema#nonNegativeInteger">0</owl:minQualifiedCardinality>
                <owl:onDataRange rdf:resource="http://www.w3.org/2001/XMLSchema#string"/>
            </owl:Restriction>
        </owl:equivalentClass>
        <owl:equivalentClass>
            <owl:Restriction>
                <owl:onProperty rdf:resource="http://www.enexis.nl/IEC-CIM#StreetAddress.postalCode"/>
                <owl:maxQualifiedCardinality rdf:datatype="http://www.w3.org/2001/XMLSchema#nonNegativeInteger">1</owl:maxQualifiedCardinality>
                <owl:onDataRange rdf:resource="http://www.w3.org/2001/XMLSchema#string"/>
            </owl:Restriction>
        </owl:equivalentClass>
        <rdfs:comment>General purpose street and postal address information.</rdfs:comment>
    </owl:Class>
    


    <!-- http://www.enexis.nl/IEC-CIM#StreetDetail -->

    <owl:Class rdf:about="http://www.enexis.nl/IEC-CIM#StreetDetail">
        <owl:equivalentClass>
            <owl:Restriction>
                <owl:onProperty rdf:resource="http://www.enexis.nl/IEC-CIM#StreetDetail.name"/>
                <owl:minQualifiedCardinality rdf:datatype="http://www.w3.org/2001/XMLSchema#nonNegativeInteger">0</owl:minQualifiedCardinality>
                <owl:onDataRange rdf:resource="http://www.w3.org/2001/XMLSchema#string"/>
            </owl:Restriction>
        </owl:equivalentClass>
        <owl:equivalentClass>
            <owl:Restriction>
                <owl:onProperty rdf:resource="http://www.enexis.nl/IEC-CIM#StreetDetail.name"/>
                <owl:maxQualifiedCardinality rdf:datatype="http://www.w3.org/2001/XMLSchema#nonNegativeInteger">1</owl:maxQualifiedCardinality>
                <owl:onDataRange rdf:resource="http://www.w3.org/2001/XMLSchema#string"/>
            </owl:Restriction>
        </owl:equivalentClass>
        <rdfs:comment>Street details, in the context of address.</rdfs:comment>
    </owl:Class>
    


    <!-- http://www.enexis.nl/IEC-CIM#TownDetail -->

    <owl:Class rdf:about="http://www.enexis.nl/IEC-CIM#TownDetail">
        <owl:equivalentClass>
            <owl:Restriction>
                <owl:onProperty rdf:resource="http://www.enexis.nl/IEC-CIM#TownDetail.name"/>
                <owl:minQualifiedCardinality rdf:datatype="http://www.w3.org/2001/XMLSchema#nonNegativeInteger">0</owl:minQualifiedCardinality>
                <owl:onDataRange rdf:resource="http://www.w3.org/2001/XMLSchema#string"/>
            </owl:Restriction>
        </owl:equivalentClass>
        <owl:equivalentClass>
            <owl:Restriction>
                <owl:onProperty rdf:resource="http://www.enexis.nl/IEC-CIM#TownDetail.name"/>
                <owl:maxQualifiedCardinality rdf:datatype="http://www.w3.org/2001/XMLSchema#nonNegativeInteger">1</owl:maxQualifiedCardinality>
                <owl:onDataRange rdf:resource="http://www.w3.org/2001/XMLSchema#string"/>
            </owl:Restriction>
        </owl:equivalentClass>
        <rdfs:comment>Town details, in the context of address.</rdfs:comment>
    </owl:Class>
    


    <!-- http://www.enexis.nl/IEC-CIM#UsagePoint -->

    <owl:Class rdf:about="http://www.enexis.nl/IEC-CIM#UsagePoint">
        <rdfs:subClassOf rdf:resource="http://www.enexis.nl/IEC-CIM#IdentifiedObject"/>
        <rdfs:comment>Logical or physical point in the network to which readings or events may be attributed. Used at the place where a physical or virtual meter may be located; however, it is not required that a meter be present.</rdfs:comment>
    </owl:Class>
    


    <!-- http://www.opengis.net/ont/geosparql#Feature -->

    <owl:Class rdf:about="http://www.opengis.net/ont/geosparql#Feature">
        <rdfs:subClassOf rdf:resource="http://www.opengis.net/ont/geosparql#SpatialObject"/>
        <owl:disjointWith rdf:resource="http://www.opengis.net/ont/geosparql#Geometry"/>
        <dc:contributor>Matthew Perry</dc:contributor>
        <dc:creator>OGC GeoSPARQL 1.0 Standard Working Group</dc:creator>
        <dc:date rdf:datatype="http://www.w3.org/2001/XMLSchema#date">2011-06-16</dc:date>
        <dc:description xml:lang="en">
      This class represents the top-level feature type. This class is 
      equivalent to GFI_Feature defined in ISO 19156:2011, and it is 
      superclass of all feature types.
    </dc:description>
        <rdfs:comment xml:lang="en">
      This class represents the top-level feature type. This class is 
      equivalent to GFI_Feature defined in ISO 19156:2011, and it is 
      superclass of all feature types.
    </rdfs:comment>
        <rdfs:isDefinedBy rdf:resource="http://www.opengis.net/ont/geosparql"/>
        <rdfs:isDefinedBy rdf:resource="http://www.opengis.net/ont/gml"/>
        <rdfs:isDefinedBy rdf:resource="http://www.opengis.net/spec/geosparql/1.0"/>
        <rdfs:label xml:lang="en">Feature</rdfs:label>
        <skos:definition xml:lang="en">
      This class represents the top-level feature type. This class is 
      equivalent to GFI_Feature defined in ISO 19156:2011, and it is 
      superclass of all feature types.
    </skos:definition>
        <skos:prefLabel xml:lang="en">Feature</skos:prefLabel>
    </owl:Class>
    


    <!-- http://www.opengis.net/ont/geosparql#Geometry -->

    <owl:Class rdf:about="http://www.opengis.net/ont/geosparql#Geometry">
        <rdfs:subClassOf rdf:resource="http://www.opengis.net/ont/geosparql#SpatialObject"/>
        <dc:contributor>Matthew Perry</dc:contributor>
        <dc:creator>OGC GeoSPARQL 1.0 Standard Working Group</dc:creator>
        <dc:date rdf:datatype="http://www.w3.org/2001/XMLSchema#date">2011-06-16</dc:date>
        <dc:description xml:lang="en">
      The class represents the top-level geometry type. This class is 
      equivalent to the UML class GM_Object defined in ISO 19107, and 
      it is superclass of all geometry types.
    </dc:description>
        <rdfs:comment xml:lang="en">
      The class represents the top-level geometry type. This class is 
      equivalent to the UML class GM_Object defined in ISO 19107, and 
      it is superclass of all geometry types.
    </rdfs:comment>
        <rdfs:isDefinedBy rdf:resource="http://www.opengis.net/ont/geosparql"/>
        <rdfs:isDefinedBy rdf:resource="http://www.opengis.net/ont/gml"/>
        <rdfs:isDefinedBy rdf:resource="http://www.opengis.net/spec/geosparql/1.0"/>
        <rdfs:label xml:lang="en">Geometry</rdfs:label>
        <skos:definition xml:lang="en">
      The class represents the top-level geometry type. This class is 
      equivalent to the UML class GM_Object defined in ISO 19107, and 
      it is superclass of all geometry types.
    </skos:definition>
        <skos:prefLabel xml:lang="en">Geometry</skos:prefLabel>
    </owl:Class>
    


    <!-- http://www.opengis.net/ont/geosparql#SpatialObject -->

    <owl:Class rdf:about="http://www.opengis.net/ont/geosparql#SpatialObject">
        <dc:contributor>Matthew Perry</dc:contributor>
        <dc:creator>OGC GeoSPARQL 1.0 Standard Working Group</dc:creator>
        <dc:date rdf:datatype="http://www.w3.org/2001/XMLSchema#date">2011-06-16</dc:date>
        <dc:description xml:lang="en">
      The class spatial-object represents everything that can have 
      a spatial representation. It is superclass of feature and geometry.
    </dc:description>
        <rdfs:comment xml:lang="en">
      The class spatial-object represents everything that can have 
      a spatial representation. It is superclass of feature and geometry.
    </rdfs:comment>
        <rdfs:isDefinedBy rdf:resource="http://www.opengis.net/ont/geosparql"/>
        <rdfs:isDefinedBy rdf:resource="http://www.opengis.net/ont/gml"/>
        <rdfs:isDefinedBy rdf:resource="http://www.opengis.net/spec/geosparql/1.0"/>
        <rdfs:label xml:lang="en">SpatialObject</rdfs:label>
        <skos:definition xml:lang="en">
      The class spatial-object represents everything that can have 
      a spatial representation. It is superclass of feature and geometry.
    </skos:definition>
        <skos:prefLabel xml:lang="en">SpatialObject</skos:prefLabel>
    </owl:Class>
    


    <!-- http://www.opengis.net/ont/sf#Point -->

    <owl:Class rdf:about="http://www.opengis.net/ont/sf#Point">
        <rdfs:subClassOf rdf:resource="http://www.opengis.net/ont/geosparql#Geometry"/>
        <rdfs:comment xml:lang="en">
A Point is a 0-dimensional geometric object and represents a single location in coordinate space. 
A Point has an x-coordinate value, a y-coordinate value. If called for by the associated Spatial Reference System, it may also have coordinate values for z and m.
The boundary of a Point is the empty set.
    </rdfs:comment>
        <rdfs:isDefinedBy rdf:resource="http://www.opengis.net/ont/sf"/>
        <rdfs:label xml:lang="en">Point</rdfs:label>
    </owl:Class>
</rdf:RDF>



<!-- Generated by the OWL API (version 4.2.5.20160517-0735) https://github.com/owlcs/owlapi -->

